Introduced a separate map T which tokens() operates on. This should fix a problem that made checking of nw invariants unsound. It also means that inhale/exhale is not used as before.

src/fi/abo/it/actortool/Prelude.scala
@@ -62,6 +62,7 @@ var M: MType;
 var C: CType;
 var R: CType;
 var I: CType;
+var T: CType;
 
 const unique this#: Actor;
 type List a = [@inttype@]a;
