src/fi/abo/it/actortool/boogie/Helper.scala
@@ -12,11 +12,11 @@ import fi.abo.it.actortool._
 
 object BMap extends Enumeration {
   type BMap = String
-  final val L = "L"
   final val C = "C"
   final val R = "R"
   final val M = "M"
   final val I = "I"
+  final val T = "T"
   final val St = "St"
   final val SqnCh = "SqnCh"
   final val SqnActor = "SqnAct"
@@ -95,19 +95,21 @@ object B {
   def C(channel: Boogie.Expr): Boogie.Expr = (VarExpr(BMap.C) apply channel)
   def R(channel: Boogie.Expr): Boogie.Expr = (VarExpr(BMap.R) apply channel)
   def I(channel: Boogie.Expr): Boogie.Expr = (VarExpr(BMap.I) apply channel)
+  def T(channel: Boogie.Expr): Boogie.Expr = (VarExpr(BMap.T) apply channel)
   
   def R(channel: String): Boogie.Expr = R(Boogie.VarExpr(channel))
   def C(channel: String): Boogie.Expr = C(Boogie.VarExpr(channel))
   def I(channel: String): Boogie.Expr = I(Boogie.VarExpr(channel))
+  def T(channel: String): Boogie.Expr = T(Boogie.VarExpr(channel))
   
-  def Credit(channel: String): Boogie.Expr = C(channel) - R(channel)
-  def Credit(channel: Boogie.Expr): Boogie.Expr = C(channel) - R(channel)
-  
-  def Read(channel: String): Boogie.Expr = R(channel)
-  def Read(channel: Boogie.Expr): Boogie.Expr = R(channel)
-  
-  def Total(channel: String)(implicit bvMode: Boolean): Boogie.Expr = C(channel)
-  def Total(channel: Boogie.Expr)(implicit bvMode: Boolean): Boogie.Expr = C(channel)
+  def Urd(channel: String): Boogie.Expr = C(channel) - R(channel)
+  def Urd(channel: Boogie.Expr): Boogie.Expr = C(channel) - R(channel)
+//  
+//  def Read(channel: String): Boogie.Expr = R(channel)
+//  def Read(channel: Boogie.Expr): Boogie.Expr = R(channel)
+//  
+//  def Total(channel: String)(implicit bvMode: Boolean): Boogie.Expr = C(channel)
+//  def Total(channel: Boogie.Expr)(implicit bvMode: Boolean): Boogie.Expr = C(channel)
   
   def SqnCh(connName: String, ind: Boogie.Expr): Boogie.Expr = SqnCh(VarExpr(connName),ind)
   def SqnCh(channel: Boogie.Expr, ind: Boogie.Expr): Boogie.Expr = (VarExpr(BMap.SqnCh) apply channel) apply ind
