tests/AddDelay.bpl
@@ -11,6 +11,7 @@ var M: MType;
 var C: CType;
 var R: CType;
 var I: CType;
+var T: CType;
 
 const unique this#: Actor;
 type List a = [int]a;
@@ -23,7 +24,7 @@ function AT#Min(x:int, y: int): int { if x <= y then x else y }
 // ---------------------------------------------------------------
 
 procedure Add#init#0()
-  modifies C, R, M, I;
+  modifies C, R, M, I, T;
 {
   var in1: Chan (int);
   var in2: Chan (int);
@@ -39,7 +40,7 @@ procedure Add#init#0()
   );
 }
 procedure Add#anon$0#1()
-  modifies C, R, M, I;
+  modifies C, R, M, I, T;
 {
   var in1: Chan (int);
   var in2: Chan (int);
@@ -68,7 +69,7 @@ procedure Add#anon$0#1()
   );
 }
 procedure Split#init#2()
-  modifies C, R, M, I;
+  modifies C, R, M, I, T;
 {
   var in: Chan (int);
   var out1: Chan (int);
@@ -87,7 +88,7 @@ procedure Split#init#2()
   );
 }
 procedure Split#anon$1#3()
-  modifies C, R, M, I;
+  modifies C, R, M, I, T;
 {
   var in: Chan (int);
   var out1: Chan (int);
@@ -121,7 +122,7 @@ procedure Split#anon$1#3()
   );
 }
 procedure Delay#init#4()
-  modifies C, R, M, I;
+  modifies C, R, M, I, T;
 {
   var in: Chan (int);
   var out: Chan (int);
@@ -137,7 +138,7 @@ procedure Delay#init#4()
   );
 }
 procedure Delay#anon$3#5()
-  modifies C, R, M, I;
+  modifies C, R, M, I, T;
 {
   var in: Chan (int);
   var out: Chan (int);
@@ -160,7 +161,7 @@ procedure Delay#anon$3#5()
   );
 }
 procedure Net#init#6()
-  modifies C, R, M, I;
+  modifies C, R, M, I, T;
 {
   var Net#add: Actor;
   var Net#del: Actor;
@@ -175,19 +176,24 @@ procedure Net#init#6()
   assume 0 <= I[Net#a];
   assume I[Net#a] <= R[Net#a];
   assume R[Net#a] <= C[Net#a];
+  assume T[Net#a] == 0;
   assume 0 <= I[Net#b];
   assume I[Net#b] <= R[Net#b];
   assume R[Net#b] <= C[Net#b];
+  assume T[Net#b] == 0;
   assume 0 <= I[Net#c];
   assume I[Net#c] <= R[Net#c];
   assume R[Net#c] <= C[Net#c];
+  assume T[Net#c] == 0;
   assume 0 <= I[Net#d];
   assume I[Net#d] <= R[Net#d];
   assume R[Net#d] <= C[Net#d];
+  assume T[Net#d] == 0;
   assume I[Net#d] == R[Net#d];
   assume 0 <= I[Net#e];
   assume I[Net#e] <= R[Net#e];
   assume R[Net#e] <= C[Net#e];
+  assume T[Net#e] == 0;
   assume C[Net#a] == 0;
   assume R[Net#a] == 0;
   assume C[Net#b] == 0;
@@ -226,15 +232,15 @@ procedure Net#init#6()
   assert {:msg "Initialization of network 'Net' might not establish the channel invariant (#23)"} I[Net#d] == I[Net#c];
   assert {:msg "Initialization of network 'Net' might not establish the channel invariant (#24)"} I[Net#e] == I[Net#c];
   I := R;
-  C[Net#b] := C[Net#b] - 1;
-  assert {:msg "35.5: The initialization might produce unspecified tokens on channel a (#25)"} (C[Net#a] - R[Net#a]) == 0;
-  assert {:msg "36.5: The initialization might produce unspecified tokens on channel b (#26)"} (C[Net#b] - R[Net#b]) == 0;
-  assert {:msg "37.5: The initialization might produce unspecified tokens on channel c (#27)"} (C[Net#c] - R[Net#c]) == 0;
-  assert {:msg "38.5: The initialization might produce unspecified tokens on channel d (#28)"} (C[Net#d] - R[Net#d]) == 0;
-  assert {:msg "39.5: The initialization might produce unspecified tokens on channel e (#29)"} (C[Net#e] - R[Net#e]) == 0;
+  T[Net#b] := T[Net#b] + 1;
+  assert {:msg "35.5: The initialization might produce unspecified tokens on channel a (#25)"} (C[Net#a] - R[Net#a]) == T[Net#a];
+  assert {:msg "36.5: The initialization might produce unspecified tokens on channel b (#26)"} (C[Net#b] - R[Net#b]) == T[Net#b];
+  assert {:msg "37.5: The initialization might produce unspecified tokens on channel c (#27)"} (C[Net#c] - R[Net#c]) == T[Net#c];
+  assert {:msg "38.5: The initialization might produce unspecified tokens on channel d (#28)"} (C[Net#d] - R[Net#d]) == T[Net#d];
+  assert {:msg "39.5: The initialization might produce unspecified tokens on channel e (#29)"} (C[Net#e] - R[Net#e]) == T[Net#e];
 }
 procedure Net##Add#anon$0#7()
-  modifies C, R, M, I;
+  modifies C, R, M, I, T;
 {
   var Net#add: Actor;
   var Net#del: Actor;
@@ -251,19 +257,24 @@ procedure Net##Add#anon$0#7()
   assume 0 <= I[Net#a];
   assume I[Net#a] <= R[Net#a];
   assume R[Net#a] <= C[Net#a];
+  assume T[Net#a] == 0;
   assume 0 <= I[Net#b];
   assume I[Net#b] <= R[Net#b];
   assume R[Net#b] <= C[Net#b];
+  assume T[Net#b] == 0;
   assume 0 <= I[Net#c];
   assume I[Net#c] <= R[Net#c];
   assume R[Net#c] <= C[Net#c];
+  assume T[Net#c] == 0;
   assume 0 <= I[Net#d];
   assume I[Net#d] <= R[Net#d];
   assume R[Net#d] <= C[Net#d];
+  assume T[Net#d] == 0;
   assume I[Net#d] == R[Net#d];
   assume 0 <= I[Net#e];
   assume I[Net#e] <= R[Net#e];
   assume R[Net#e] <= C[Net#e];
+  assume T[Net#e] == 0;
   assume M[Net#b][0] == 0;
   assume 0 <= M[Net#b][I[Net#b]];
   assume I[Net#c] == I[Net#a];
@@ -295,9 +306,9 @@ procedure Net##Add#anon$0#7()
   assume (forall idx$: int :: 
     (0 <= idx$) && (idx$ < C[Net#c]) ==> (M[Net#c][idx$] == (M[Net#a][idx$] + M[Net#b][idx$]))
   );
-  in1#i := M[Net#a][R[Net#a]];
+  in1#i := M[Net#a][C[Net#a] - R[Net#a]];
   R[Net#a] := R[Net#a] + 1;
-  in2#j := M[Net#b][R[Net#b]];
+  in2#j := M[Net#b][C[Net#b] - R[Net#b]];
   R[Net#b] := R[Net#b] + 1;
   M[Net#c][C[Net#c]] := in1#i + in2#j;
   C[Net#c] := C[Net#c] + 1;
@@ -332,7 +343,7 @@ procedure Net##Add#anon$0#7()
   assert {:msg "Action at 2.3 ('anon$0') for actor instance 'add' might not preserve the channel invariant (#36)"} I[Net#e] == I[Net#c];
 }
 procedure Net##Delay#anon$3#8()
-  modifies C, R, M, I;
+  modifies C, R, M, I, T;
 {
   var Net#add: Actor;
   var Net#del: Actor;
@@ -348,19 +359,24 @@ procedure Net##Delay#anon$3#8()
   assume 0 <= I[Net#a];
   assume I[Net#a] <= R[Net#a];
   assume R[Net#a] <= C[Net#a];
+  assume T[Net#a] == 0;
   assume 0 <= I[Net#b];
   assume I[Net#b] <= R[Net#b];
   assume R[Net#b] <= C[Net#b];
+  assume T[Net#b] == 0;
   assume 0 <= I[Net#c];
   assume I[Net#c] <= R[Net#c];
   assume R[Net#c] <= C[Net#c];
+  assume T[Net#c] == 0;
   assume 0 <= I[Net#d];
   assume I[Net#d] <= R[Net#d];
   assume R[Net#d] <= C[Net#d];
+  assume T[Net#d] == 0;
   assume I[Net#d] == R[Net#d];
   assume 0 <= I[Net#e];
   assume I[Net#e] <= R[Net#e];
   assume R[Net#e] <= C[Net#e];
+  assume T[Net#e] == 0;
   assume M[Net#b][0] == 0;
   assume 0 <= M[Net#b][I[Net#b]];
   assume I[Net#c] == I[Net#a];
@@ -391,7 +407,7 @@ procedure Net##Delay#anon$3#8()
   assume (forall idx$: int :: 
     (1 <= idx$) && (idx$ < C[Net#b]) ==> (M[Net#b][idx$] == M[Net#e][idx$ - 1])
   );
-  in#i := M[Net#e][R[Net#e]];
+  in#i := M[Net#e][C[Net#e] - R[Net#e]];
   R[Net#e] := R[Net#e] + 1;
   M[Net#b][C[Net#b]] := in#i;
   C[Net#b] := C[Net#b] + 1;
@@ -425,7 +441,7 @@ procedure Net##Delay#anon$3#8()
   assert {:msg "Action at 12.3 ('anon$3') for actor instance 'del' might not preserve the channel invariant (#43)"} I[Net#e] == I[Net#c];
 }
 procedure Net##Split#anon$1#9()
-  modifies C, R, M, I;
+  modifies C, R, M, I, T;
 {
   var Net#add: Actor;
   var Net#del: Actor;
@@ -441,19 +457,24 @@ procedure Net##Split#anon$1#9()
   assume 0 <= I[Net#a];
   assume I[Net#a] <= R[Net#a];
   assume R[Net#a] <= C[Net#a];
+  assume T[Net#a] == 0;
   assume 0 <= I[Net#b];
   assume I[Net#b] <= R[Net#b];
   assume R[Net#b] <= C[Net#b];
+  assume T[Net#b] == 0;
   assume 0 <= I[Net#c];
   assume I[Net#c] <= R[Net#c];
   assume R[Net#c] <= C[Net#c];
+  assume T[Net#c] == 0;
   assume 0 <= I[Net#d];
   assume I[Net#d] <= R[Net#d];
   assume R[Net#d] <= C[Net#d];
+  assume T[Net#d] == 0;
   assume I[Net#d] == R[Net#d];
   assume 0 <= I[Net#e];
   assume I[Net#e] <= R[Net#e];
   assume R[Net#e] <= C[Net#e];
+  assume T[Net#e] == 0;
   assume M[Net#b][0] == 0;
   assume 0 <= M[Net#b][I[Net#b]];
   assume I[Net#c] == I[Net#a];
@@ -488,7 +509,7 @@ procedure Net##Split#anon$1#9()
   assume (forall idx$: int :: 
     (0 <= idx$) && (idx$ < C[Net#e]) ==> (M[Net#e][idx$] == M[Net#c][idx$])
   );
-  in#i := M[Net#c][R[Net#c]];
+  in#i := M[Net#c][C[Net#c] - R[Net#c]];
   R[Net#c] := R[Net#c] + 1;
   M[Net#d][C[Net#d]] := in#i;
   C[Net#d] := C[Net#d] + 1;
@@ -528,7 +549,7 @@ procedure Net##Split#anon$1#9()
   assert {:msg "Action at 6.3 ('anon$1') for actor instance 'spl' might not preserve the channel invariant (#50)"} I[Net#e] == I[Net#c];
 }
 procedure Net#entry()
-  modifies C, R, M, I;
+  modifies C, R, M, I, T;
 {
   var Net#add: Actor;
   var Net#del: Actor;
@@ -543,25 +564,30 @@ procedure Net#entry()
   assume 0 <= I[Net#a];
   assume I[Net#a] <= R[Net#a];
   assume R[Net#a] <= C[Net#a];
+  assume T[Net#a] == 0;
   assume 0 <= I[Net#b];
   assume I[Net#b] <= R[Net#b];
   assume R[Net#b] <= C[Net#b];
+  assume T[Net#b] == 0;
   assume 0 <= I[Net#c];
   assume I[Net#c] <= R[Net#c];
   assume R[Net#c] <= C[Net#c];
+  assume T[Net#c] == 0;
   assume 0 <= I[Net#d];
   assume I[Net#d] <= R[Net#d];
   assume R[Net#d] <= C[Net#d];
+  assume T[Net#d] == 0;
   assume I[Net#d] == R[Net#d];
   assume 0 <= I[Net#e];
   assume I[Net#e] <= R[Net#e];
   assume R[Net#e] <= C[Net#e];
+  assume T[Net#e] == 0;
   assume C[Net#a] == R[Net#a];
   assume C[Net#b] == R[Net#b];
   assume C[Net#c] == R[Net#c];
   assume C[Net#d] == R[Net#d];
   assume C[Net#e] == R[Net#e];
-  C[Net#b] := C[Net#b] + 1;
+  T[Net#b] := T[Net#b] + 1;
   assume M[Net#b][0] == 0;
   assume 0 <= M[Net#b][I[Net#b]];
   assume I[Net#c] == I[Net#a];
@@ -592,7 +618,7 @@ procedure Net#entry()
   assert {:msg "15.1: Sub-actors in the network might fire without network input. This is not permitted. (#53)"} !(1 <= (C[Net#c] - R[Net#c]));
 }
 procedure Net#anon$4#input#in#10()
-  modifies C, R, M, I;
+  modifies C, R, M, I, T;
 {
   var Net#add: Actor;
   var Net#del: Actor;
@@ -607,19 +633,24 @@ procedure Net#anon$4#input#in#10()
   assume 0 <= I[Net#a];
   assume I[Net#a] <= R[Net#a];
   assume R[Net#a] <= C[Net#a];
+  assume T[Net#a] == 0;
   assume 0 <= I[Net#b];
   assume I[Net#b] <= R[Net#b];
   assume R[Net#b] <= C[Net#b];
+  assume T[Net#b] == 0;
   assume 0 <= I[Net#c];
   assume I[Net#c] <= R[Net#c];
   assume R[Net#c] <= C[Net#c];
+  assume T[Net#c] == 0;
   assume 0 <= I[Net#d];
   assume I[Net#d] <= R[Net#d];
   assume R[Net#d] <= C[Net#d];
+  assume T[Net#d] == 0;
   assume I[Net#d] == R[Net#d];
   assume 0 <= I[Net#e];
   assume I[Net#e] <= R[Net#e];
   assume R[Net#e] <= C[Net#e];
+  assume T[Net#e] == 0;
   assume (C[Net#a] - I[Net#a]) < 1;
   assume M[Net#b][0] == 0;
   assume 0 <= M[Net#b][I[Net#b]];
@@ -658,7 +689,7 @@ procedure Net#anon$4#input#in#10()
   assert {:msg "18.14: Channel invariant might be falsified by network input (#61)"} 0 <= M[Net#a][I[Net#a]];
 }
 procedure Net#anon$4#exit#11()
-  modifies C, R, M, I;
+  modifies C, R, M, I, T;
 {
   var Net#add: Actor;
   var Net#del: Actor;
@@ -673,19 +704,24 @@ procedure Net#anon$4#exit#11()
   assume 0 <= I[Net#a];
   assume I[Net#a] <= R[Net#a];
   assume R[Net#a] <= C[Net#a];
+  assume T[Net#a] == 0;
   assume 0 <= I[Net#b];
   assume I[Net#b] <= R[Net#b];
   assume R[Net#b] <= C[Net#b];
+  assume T[Net#b] == 0;
   assume 0 <= I[Net#c];
   assume I[Net#c] <= R[Net#c];
   assume R[Net#c] <= C[Net#c];
+  assume T[Net#c] == 0;
   assume 0 <= I[Net#d];
   assume I[Net#d] <= R[Net#d];
   assume R[Net#d] <= C[Net#d];
+  assume T[Net#d] == 0;
   assume I[Net#d] == R[Net#d];
   assume 0 <= I[Net#e];
   assume I[Net#e] <= R[Net#e];
   assume R[Net#e] <= C[Net#e];
+  assume T[Net#e] == 0;
   assume M[Net#b][0] == 0;
   assume 0 <= M[Net#b][I[Net#b]];
   assume I[Net#c] == I[Net#a];
@@ -728,10 +764,10 @@ procedure Net#anon$4#exit#11()
   assert {:msg "The network might not preserve the channel invariant (#69)"} I[Net#b] == I[Net#e];
   assert {:msg "The network might not preserve the channel invariant (#70)"} I[Net#d] == I[Net#c];
   assert {:msg "The network might not preserve the channel invariant (#71)"} I[Net#e] == I[Net#c];
-  C[Net#b] := C[Net#b] - 1;
-  assert {:msg "17.3: The network might leave unread tokens on channel a (#72)"} C[Net#a] == R[Net#a];
-  assert {:msg "17.3: The network might leave unread tokens on channel b (#73)"} C[Net#b] == R[Net#b];
-  assert {:msg "17.3: The network might leave unread tokens on channel c (#74)"} C[Net#c] == R[Net#c];
-  assert {:msg "17.3: The network might not produce the specified number of tokens on output out (#75)"} C[Net#d] == R[Net#d];
-  assert {:msg "17.3: The network might leave unread tokens on channel e (#76)"} C[Net#e] == R[Net#e];
+  T[Net#b] := T[Net#b] + 1;
+  assert {:msg "17.3: The network might leave unread tokens on channel a (#72)"} (C[Net#a] - R[Net#a]) == T[Net#a];
+  assert {:msg "17.3: The network might leave unread tokens on channel b (#73)"} (C[Net#b] - R[Net#b]) == T[Net#b];
+  assert {:msg "17.3: The network might leave unread tokens on channel c (#74)"} (C[Net#c] - R[Net#c]) == T[Net#c];
+  assert {:msg "17.3: The network might not produce the specified number of tokens on output out (#75)"} (C[Net#d] - R[Net#d]) == T[Net#d];
+  assert {:msg "17.3: The network might leave unread tokens on channel e (#76)"} (C[Net#e] - R[Net#e]) == T[Net#e];
 }
